Specification for SPARKLE 384/512

specs/Spec.SPARKLE.fst
@@ -52,6 +52,49 @@ let m2 x y =
   let w1 = y1 ^. lv in
   (t0, w0), (t1, w1)
 
+val m3: branch -> branch -> branch -> Tot (branch & branch & branch)
+let m3 x y z =
+  let x0 = fst x in
+  let y0 = snd x in
+  let x1 = fst y in
+  let y1 = snd y in
+  let x2 = fst z in
+  let y2 = snd z in
+  let u = y0 ^. y1 ^. y2 in
+  let v = x0 ^. x1 ^. x2 in
+  let lu = l1 u in
+  let lv = l1 v in
+  let t0 = x0 ^. lu in
+  let t1 = x1 ^. lu in
+  let t2 = x2 ^. lu in
+  let w0 = y0 ^. lv in
+  let w1 = y1 ^. lv in
+  let w2 = y2 ^. lv in
+  (t0, w0), (t1, w1), (t2, w2)
+
+val m4: branch -> branch -> branch -> branch -> Tot (branch & branch & branch & branch)
+let m4 x y z z2 =
+  let x0 = fst x in
+  let y0 = snd x in
+  let x1 = fst y in
+  let y1 = snd y in
+  let x2 = fst z in
+  let y2 = snd z in
+  let x3 = fst z2 in
+  let y3 = snd z2 in
+  let u = y0 ^. y1 ^. y2 ^. y3 in
+  let v = x0 ^. x1 ^. x2 ^. x3 in
+  let lu = l1 u in
+  let lv = l1 v in
+  let t0 = x0 ^. lu in
+  let t1 = x1 ^. lu in
+  let t2 = x2 ^. lu in
+  let t3 = x3 ^. lu in
+  let w0 = y0 ^. lv in
+  let w1 = y1 ^. lv in
+  let w2 = y2 ^. lv in
+  let w3 = y3 ^. lv in
+  (t0, w0), (t1, w1), (t2, w2), (t3, w3)
 
 val l4: branch -> branch -> branch -> branch -> Tot (branch & branch & branch & branch)
 let l4 b0 b1 b2 b3 =
@@ -59,6 +102,23 @@ let l4 b0 b1 b2 b3 =
   let o0 = (fst b3 ^. fst p1), (snd b3 ^. snd p1) in
   let o1 = (fst b2 ^. fst p0), (snd b2 ^. snd p0) in
   (o0, o1, b0, b1)
+
+val l6: branch -> branch -> branch -> branch -> branch -> branch -> Tot (branch & branch & branch & branch & branch & branch)
+let l6 b0 b1 b2 b3 b4 b5 =
+  let (p0, p1, p2) = m3 b0 b1 b2 in
+  let o0 = (fst b4 ^. fst p1), (snd b4 ^. snd p1) in
+  let o1 = (fst b5 ^. fst p2), (snd b5 ^. snd p2) in
+  let o2 = (fst b3 ^. fst p0), (snd b3 ^. snd p0) in
+  (o0, o1, o2, b0, b1, b2)
+
+val l8: branch -> branch -> branch -> branch -> branch -> branch -> branch -> branch -> Tot (branch & branch & branch & branch & branch & branch & branch & branch)
+let l8 b0 b1 b2 b3 b4 b5 b6 b7 =
+  let (p0, p1, p2, p3) = m4 b0 b1 b2 b3 in
+  let o0 = (fst b5 ^. fst p1), (snd b5 ^. snd p1) in
+  let o1 = (fst b6 ^. fst p2), (snd b6 ^. snd p2) in
+  let o2 = (fst b7 ^. fst p3), (snd b7 ^. snd p3) in
+  let o3 = (fst b4 ^. fst p0), (snd b4 ^. snd p0) in
+  (o0, o1, o2, o3, b0, b1, b2, b3)
 
 
 let size_word: size_nat = 4
@@ -76,13 +136,13 @@ let rcon_list: l:List.Tot.llist uint32 vsize_rcon =
 
 let rcon: lseq uint32 vsize_rcon  = createL rcon_list
 
-val add: i:size_nat -> branch -> branch -> branch -> branch -> Tot (branch & branch & branch & branch)
-let add i b0 b1 b2 b3 =
+val add: i:size_nat -> branch -> branch -> Tot (branch & branch)
+let add i b0 b1 =
   let y0 = snd b0 in
   let y1 = snd b1 in
   let y0 = y0 ^. rcon.[(i % vsize_rcon)] in
   let y1 = y1 ^. (u32 i) in
-  (b0, b1, b2, b3)
+  (b0, b1)
 
 
 val sparkle256: steps:size_nat -> lbytes 32 -> Tot (lbytes 32)
@@ -111,7 +171,7 @@ let sparkle256 steps input =
 
   let (b0, b1, b2, b3) =
     repeati steps (fun i (b0,b1,b2,b3) ->
-    let (b0,b1,b2,b3) = add i b0 b1 b2 b3 in
+    let (b0,b1) = add i b0 b1 in
     let b0 = arx rcon.[0] b0 in
     let b1 = arx rcon.[1] b1 in
     let b2 = arx rcon.[2] b2 in
@@ -142,4 +202,192 @@ let sparkle256 steps input =
   let input = update_sub input (5 * size_word) size_word by2 in
   let input = update_sub input (6 * size_word) size_word bx3 in
   let input = update_sub input (7 * size_word) size_word by3 in
+  input
+
+#set-options "--z3rlimit 10"
+
+val sparkle384: steps:size_nat -> lbytes 48 -> Tot (lbytes 48)
+let sparkle384 steps input =
+  let bx0 = sub input 0 size_word in
+  let by0 = sub input (1 * size_word) size_word in
+  let bx1 = sub input (2 * size_word) size_word in
+  let by1 = sub input (3 * size_word) size_word in
+  let bx2 = sub input (4 * size_word) size_word in
+  let by2 = sub input (5 * size_word) size_word in
+  let bx3 = sub input (6 * size_word) size_word in
+  let by3 = sub input (7 * size_word) size_word in
+  let bx4 = sub input (8 * size_word) size_word in
+  let by4 = sub input (9 * size_word) size_word in
+  let bx5 = sub input (10 * size_word) size_word in
+  let by5 = sub input (11 * size_word) size_word in
+  let x0 = uint_from_bytes_le bx0 in
+  let y0 = uint_from_bytes_le by0 in
+  let x1 = uint_from_bytes_le bx1 in
+  let y1 = uint_from_bytes_le by1 in
+  let x2 = uint_from_bytes_le bx2 in
+  let y2 = uint_from_bytes_le by2 in
+  let x3 = uint_from_bytes_le bx3 in
+  let y3 = uint_from_bytes_le by3 in
+  let x4 = uint_from_bytes_le bx4 in
+  let y4 = uint_from_bytes_le by4 in
+  let x5 = uint_from_bytes_le bx5 in
+  let y5 = uint_from_bytes_le by5 in
+
+  let b0 = x0, y0 in
+  let b1 = x1, y1 in
+  let b2 = x2, y2 in
+  let b3 = x3, y3 in
+  let b4 = x4, y4 in
+  let b5 = x5, y5 in
+
+  let (b0,b1,b2,b3,b4,b5) =
+    repeati steps (fun i (b0,b1,b2,b3,b4,b5) ->
+    let (b0,b1) = add i b0 b1 in
+    let b0 = arx rcon.[0] b0 in
+    let b1 = arx rcon.[1] b1 in
+    let b2 = arx rcon.[2] b2 in
+    let b3 = arx rcon.[3] b3 in
+    let b4 = arx rcon.[4] b4 in
+    let b5 = arx rcon.[5] b5 in
+    let b0,b1,b2,b3,b4,b5 = l6 b0 b1 b2 b3 b4 b5 in
+    (b0,b1,b2,b3,b4,b5)
+  ) (b0,b1,b2,b3,b4,b5)
+  in
+
+  let x0, y0 = b0 in
+  let x1, y1 = b1 in
+  let x2, y2 = b2 in
+  let x3, y3 = b3 in
+  let x4, y4 = b4 in
+  let x5, y5 = b5 in
+
+  let bx0 = uint_to_bytes_be x0 in
+  let by0 = uint_to_bytes_be y0 in
+  let bx1 = uint_to_bytes_be x1 in
+  let by1 = uint_to_bytes_be y1 in
+  let bx2 = uint_to_bytes_be x2 in
+  let by2 = uint_to_bytes_be y2 in
+  let bx3 = uint_to_bytes_be x3 in
+  let by3 = uint_to_bytes_be y3 in
+  let bx4 = uint_to_bytes_be x4 in
+  let by4 = uint_to_bytes_be y4 in
+  let bx5 = uint_to_bytes_be x5 in
+  let by5 = uint_to_bytes_be y5 in
+  let input = update_sub input 0 size_word bx0 in
+  let input = update_sub input (1 * size_word) size_word by0 in
+  let input = update_sub input (2 * size_word) size_word bx1 in
+  let input = update_sub input (3 * size_word) size_word by1 in
+  let input = update_sub input (4 * size_word) size_word bx2 in
+  let input = update_sub input (5 * size_word) size_word by2 in
+  let input = update_sub input (6 * size_word) size_word bx3 in
+  let input = update_sub input (7 * size_word) size_word by3 in
+  let input = update_sub input (8 * size_word) size_word bx4 in
+  let input = update_sub input (9 * size_word) size_word by4 in
+  let input = update_sub input (10 * size_word) size_word bx5 in
+  let input = update_sub input (11 * size_word) size_word by5 in
+  input
+
+val sparkle512: steps:size_nat -> lbytes 64 -> Tot (lbytes 64)
+let sparkle512 steps input =
+  let bx0 = sub input 0 size_word in
+  let by0 = sub input (1 * size_word) size_word in
+  let bx1 = sub input (2 * size_word) size_word in
+  let by1 = sub input (3 * size_word) size_word in
+  let bx2 = sub input (4 * size_word) size_word in
+  let by2 = sub input (5 * size_word) size_word in
+  let bx3 = sub input (6 * size_word) size_word in
+  let by3 = sub input (7 * size_word) size_word in
+  let bx4 = sub input (8 * size_word) size_word in
+  let by4 = sub input (9 * size_word) size_word in
+  let bx5 = sub input (10 * size_word) size_word in
+  let by5 = sub input (11 * size_word) size_word in
+  let bx6 = sub input (12 * size_word) size_word in
+  let by6 = sub input (13 * size_word) size_word in
+  let bx7 = sub input (14 * size_word) size_word in
+  let by7 = sub input (15 * size_word) size_word in
+  let x0 = uint_from_bytes_le bx0 in
+  let y0 = uint_from_bytes_le by0 in
+  let x1 = uint_from_bytes_le bx1 in
+  let y1 = uint_from_bytes_le by1 in
+  let x2 = uint_from_bytes_le bx2 in
+  let y2 = uint_from_bytes_le by2 in
+  let x3 = uint_from_bytes_le bx3 in
+  let y3 = uint_from_bytes_le by3 in
+  let x4 = uint_from_bytes_le bx4 in
+  let y4 = uint_from_bytes_le by4 in
+  let x5 = uint_from_bytes_le bx5 in
+  let y5 = uint_from_bytes_le by5 in
+  let x6 = uint_from_bytes_le bx6 in
+  let y6 = uint_from_bytes_le by6 in
+  let x7 = uint_from_bytes_le bx7 in
+  let y7 = uint_from_bytes_le by7 in
+
+  let b0 = x0, y0 in
+  let b1 = x1, y1 in
+  let b2 = x2, y2 in
+  let b3 = x3, y3 in
+  let b4 = x4, y4 in
+  let b5 = x5, y5 in
+  let b6 = x6, y6 in
+  let b6 = x6, y6 in
+  let b7 = x7, y7 in
+  let b7 = x7, y7 in
+
+  let (b0,b1,b2,b3,b4,b5,b6,b7) =
+    repeati steps (fun i (b0,b1,b2,b3,b4,b5,b6,b7) ->
+    let (b0,b1) = add i b0 b1 in
+    let b0 = arx rcon.[0] b0 in
+    let b1 = arx rcon.[1] b1 in
+    let b2 = arx rcon.[2] b2 in
+    let b3 = arx rcon.[3] b3 in
+    let b4 = arx rcon.[4] b4 in
+    let b5 = arx rcon.[5] b5 in
+    let b6 = arx rcon.[6] b6 in
+    let b7 = arx rcon.[7] b7 in
+    let b0,b1,b2,b3,b4,b5,b7,b8 = l8 b0 b1 b2 b3 b4 b5 b6 b7 in
+    (b0,b1,b2,b3,b4,b5,b6,b7)
+  ) (b0,b1,b2,b3,b4,b5,b7,b7)
+  in
+
+  let x0, y0 = b0 in
+  let x1, y1 = b1 in
+  let x2, y2 = b2 in
+  let x3, y3 = b3 in
+  let x4, y4 = b4 in
+  let x5, y5 = b5 in
+  let x6, y6 = b6 in
+  let x7, y7 = b7 in
+
+  let bx0 = uint_to_bytes_be x0 in
+  let by0 = uint_to_bytes_be y0 in
+  let bx1 = uint_to_bytes_be x1 in
+  let by1 = uint_to_bytes_be y1 in
+  let bx2 = uint_to_bytes_be x2 in
+  let by2 = uint_to_bytes_be y2 in
+  let bx3 = uint_to_bytes_be x3 in
+  let by3 = uint_to_bytes_be y3 in
+  let bx4 = uint_to_bytes_be x4 in
+  let by4 = uint_to_bytes_be y4 in
+  let bx5 = uint_to_bytes_be x5 in
+  let by5 = uint_to_bytes_be y5 in
+  let bx6 = uint_to_bytes_be x6 in
+  let by6 = uint_to_bytes_be y6 in
+  let bx7 = uint_to_bytes_be x7 in
+  let by7 = uint_to_bytes_be y7 in
+  let input = update_sub input 0 size_word bx0 in
+  let input = update_sub input (1 * size_word) size_word by0 in
+  let input = update_sub input (2 * size_word) size_word bx1 in
+  let input = update_sub input (3 * size_word) size_word by1 in
+  let input = update_sub input (4 * size_word) size_word bx2 in
+  let input = update_sub input (5 * size_word) size_word by2 in
+  let input = update_sub input (6 * size_word) size_word bx3 in
+  let input = update_sub input (7 * size_word) size_word by3 in
+  let input = update_sub input (8 * size_word) size_word bx4 in
+  let input = update_sub input (9 * size_word) size_word by4 in
+  let input = update_sub input (10 * size_word) size_word bx5 in
+  let input = update_sub input (11 * size_word) size_word by5 in
+  let input = update_sub input (12 * size_word) size_word bx6 in
+  let input = update_sub input (13 * size_word) size_word by6 in
+  let input = update_sub input (14 * size_word) size_word bx7 in
+  let input = update_sub input (15 * size_word) size_word by7 in
   input
